Infix Completeness proof

IGrammar.v
@@ -167,4 +167,33 @@ Fixpoint fix_tree {L O} (pr : drules O) t : parse_tree L O :=
   | INode t1 o t2 => linsert pr t1 o (fix_tree pr t2)
   end.
 
+Fixpoint simpleton_linsert {L O} (pr : drules O) t1 o t2 : parse_tree L O :=
+  match t2 with
+  | ANode l2 => INode t1 o (ANode l2)
+  | INode t21 o2 t22 =>
+      if is_conflict_pattern pr (CR o o2)
+      then INode (simpleton_linsert pr t1 o t21) o2 t22
+      else INode t1 o (INode t21 o2 t22)
+  end.
+
+Inductive complete_conflicts {O} (Q : tree_pattern O -> Prop) : tree_pattern O -> Prop :=
+  | QSelf q :
+      Q q ->
+      complete_conflicts Q q
+  | CR_CL o1 o2 :
+      ~ Q (CR o1 o2) ->
+      complete_conflicts Q (CL o2 o1)
+  | CL_CR o1 o2 :
+      ~ Q (CL o1 o2) ->
+      complete_conflicts Q (CR o2 o1).
+
+Definition complete_tree {L O} (Q : tree_pattern O -> Prop) (t : parse_tree L O) : Prop :=
+  conflict_free (complete_conflicts Q) t.
+
+Fixpoint tree_size {L O} (t : parse_tree L O) : nat :=
+  match t with
+  | ANode l => 0
+  | INode t1 o t2 => S (tree_size t1 + tree_size t2)
+  end.
+
 End IGrammarFix.
